Inhabit/Examples.lean
@@ -1,0 +1,20 @@
+import Inhabit.Resolution
+
+-- Inferences
+def trivial_inf : Inference := ⟨[], .top⟩
+
+theorem trivial_sound : trivial_inf.sound := by
+  intros s i h
+  trivial
+
+def contra_inf : Inference := ⟨[.btm], .var "p"⟩
+
+theorem contra_sound : contra_inf.sound := by
+  intros s i h
+  simp [contra_inf] at h
+
+def modpon_inf : Inference := ⟨[.var "p", .imp (.var "p") (.var "q")], .var "q"⟩
+
+theorem modpon_sound : modpon_inf.sound := by
+  intros i h
+  simp_all [modpon_inf]
